rupicola/EquivRel.fst
@@ -2,37 +2,36 @@ module EquivRel
 
 open FStar.FunctionalExtensionality
 
-type fs_env #g g_card =
-  restricted_t (x:var{x < g_card}) (fun x -> elab_typ (Some?.v (g x)))
+type fs_env g =
+  restricted_t (x:var{Some? (g x)}) (fun x -> elab_typ (Some?.v (g x)))
 
-let fs_empty : fs_env #empty 0 =
+let fs_empty : fs_env empty =
   on_dom
-    (x:var{x < 0})
+    (x:var{Some? (empty x)})
     #(fun x -> elab_typ (Some?.v (empty x)))
     (fun _ -> assert False)
 
-let get_v #g #g_card fs_s i =
-  fs_s (fs_to_var g_card i)
+let get_v #g fs_s x = fs_s x
 
-let fs_extend #g #g_card fs_s #t fs_v =
+let fs_extend #g fs_s #t fs_v =
   on_dom
-    (x:var{x < g_card+1})
+    (x:var{Some? ((extend t g) x)})
     #(fun x -> elab_typ (Some?.v ((extend t g) x)))
     (fun y ->
       if y = 0 then fs_v else fs_s (y-1))
 
-let fs_shrink #t #g #g_card fs_s =
+let fs_shrink #t #g fs_s =
   on_dom
-    (x:var{x < g_card})
+    (x:var{Some? (g x)})
     #(fun x -> elab_typ (Some?.v (g x)))
     (fun y -> fs_s (y+1))
 
 let lem_fs_extend fs_s v = ()
 let lem_fs_shrink fs_s = ()
 
-let shrink_extend_inverse #g #g_card fs_s #t v =
-  let fs_s' : fs_env g_card = fs_shrink (fs_extend fs_s v) in
+let shrink_extend_inverse #g fs_s #t v =
+  let fs_s' : fs_env g = fs_shrink (fs_extend fs_s v) in
   assert (forall x. fs_s' x == fs_s x);
   assert (feq fs_s' fs_s);
-  extensionality (x:var{x < g_card}) (fun x -> elab_typ (Some?.v (g x))) fs_s' fs_s;
+  extensionality (x:var{Some? (g x)}) (fun x -> elab_typ (Some?.v (g x))) fs_s' fs_s;
   assert (fs_s' == fs_s)
