rupicola/EquivRel.fsti
@@ -32,24 +32,21 @@ let lem_values_are_expressions t fs_e e : (** lemma used by Amal **)
   Lemma (requires t ∋ (fs_e, e))
         (ensures  t ⦂ (fs_e, e)) = admit ()
 
-type env_card (g:env) =
-  g_card:nat{forall (i:nat). i < g_card ==> Some? (g i)}
-
 (** STLC Evaluation Environment : variable -> value **)
 
-let gsub (g:env) (g_card:env_card g) (b:bool{b ==> (forall x. None? (g x))}) =
+let gsub (g:env) (b:bool{b ==> (forall x. None? (g x))}) =
   s:(sub b){
-    forall (x:var). Some? (g x) ==>  x < g_card /\ is_value (s x)}
+    forall (x:var). Some? (g x) ==>  is_value (s x)}
 
-let gsub_empty : gsub empty 0 true =
+let gsub_empty : gsub empty true =
   (fun v -> EVar v)
 
-let gsub_extend (#g:env) #b #g_card (s:gsub g g_card b) (t:typ) (v:value) : gsub (extend t g) (g_card+1) false =
+let gsub_extend (#g:env) #b (s:gsub g b) (t:typ) (v:value) : gsub (extend t g) false =
   let f = fun (y:var) -> if y = 0 then v else s (y-1) in
   introduce exists (x:var). ~(EVar? (f x)) with 0 and ();
   f
 
-let gsubst (#g:env) #b #g_card (s:gsub g b g_card) (e:exp{fv_in_env g e}) : closed_exp =
+let gsubst (#g:env) #b (s:gsub g b) (e:exp{fv_in_env g e}) : closed_exp =
   lem_subst_freevars_closes_exp s e 0;
   subst s e
 
@@ -68,84 +65,76 @@ let lem_gsubst_empty (e:closed_exp) : Lemma (gsubst gsub_empty e == e)
     - we wrap f to a function that takes as argument an F* evaluation environment
       that was extended to contain a value of type 'a
     - we take the value from the environment to open f:
-        fun fs_s -> f (get_v fs_s |fs_s|)
+        fun fs_s -> f (get_v fs_s 0)
 
     What is cool about this is to define compilation to STLC the environment is abstract.
  **)
 
-(** The deBrujin index is inverse to the index in F* env **)
-let var_to_fs (g_card:nat) (x:var{x < g_card}) : (i:nat{i < g_card}) = g_card-x-1
-let fs_to_var (g_card:nat) (i:nat{i < g_card}) : var = g_card-i-1
-let lem_inverse (g_card:nat) (x:var{x < g_card}) : Lemma (fs_to_var g_card (var_to_fs g_card x) == x) = ()
-let lem_inverse' (g_card:nat) (i:var{i < g_card}) : Lemma (var_to_fs g_card (fs_to_var g_card i) == i) = ()
+val fs_env (g:env) : Type u#0
+val fs_empty : fs_env empty
+val get_v : #g:env -> fs_env g -> x:var{Some? (g x)} -> elab_typ (Some?.v (g x))
+val fs_extend : #g:env -> fs_s:fs_env g -> #t:typ -> elab_typ t -> fs_env (extend t g)
+val fs_shrink : #t:typ -> #g:env -> fs_env (extend t g) -> fs_env g
 
-
-val fs_env #g (g_card:env_card g) : Type u#0 (** having such an env is even possible in practice? what would its universe be? **)
-val fs_empty : fs_env #empty 0
-val get_v : #g:_ -> #g_card:env_card g -> fs_env g_card -> i:nat{i < g_card} -> elab_typ (Some?.v (g (fs_to_var g_card i)))
-val fs_extend : #g:_ -> #g_card:env_card g -> fs_s:fs_env g_card -> #t:typ -> elab_typ t -> fs_env #(extend t g) (g_card+1)
-val fs_shrink : #t:typ -> #g:_ -> #g_card:env_card g -> fs_env #(extend t g) (g_card+1) -> fs_env #g g_card
-
-val lem_fs_extend #g (#g_card:env_card g) (fs_s:fs_env g_card) #t (v:elab_typ t) : Lemma (
-  (forall (i:nat). i < g_card ==> get_v fs_s i == get_v (fs_extend fs_s v) i) /\
-  get_v (fs_extend fs_s v) g_card == v)
+val lem_fs_extend #g (fs_s:fs_env g) #t (v:elab_typ t) : Lemma (
+  (forall (x:var). Some? (g x) ==>  get_v fs_s x == get_v (fs_extend fs_s v) (x+1)) /\
+  get_v (fs_extend fs_s v) 0 == v)
   [SMTPat (fs_extend fs_s v)]
 
-val lem_fs_shrink #g (#g_card:env_card g) #t (fs_s:fs_env #(extend t g) (g_card+1)) : Lemma (
-  (forall (i:nat). i < g_card ==> get_v fs_s i == get_v (fs_shrink fs_s) i))
+val lem_fs_shrink #g #t (fs_s:fs_env (extend t g)) : Lemma (
+  (forall (x:var). Some? (g x) ==>  get_v fs_s (x+1) == get_v (fs_shrink fs_s) x))
   [SMTPat (fs_shrink fs_s)]
 
-val shrink_extend_inverse #g (#g_card:env_card g) (fs_s:fs_env g_card) #t (x:elab_typ t) : Lemma (fs_shrink (fs_extend fs_s x) == fs_s)
+val shrink_extend_inverse #g (fs_s:fs_env g) #t (x:elab_typ t) : Lemma (fs_shrink (fs_extend fs_s x) == fs_s)
   [SMTPat (fs_shrink (fs_extend fs_s x))]
 
-let (∽) (#g:env) #b #g_card (s:gsub g g_card b) (fs_s:fs_env g_card) : Type0 =
+let (∽) (#g:env) #b (s:gsub g b) (fs_s:fs_env g) : Type0 =
   forall (x:var). Some? (g x) ==>
-    Some?.v (g x) ∋ (get_v fs_s (var_to_fs g_card x), s x)
+    Some?.v (g x) ∋ (get_v fs_s x, s x)
 
 (** Cross Language Binary Logical Relation between F* and STLC expressions
      for __open terms__. **)
-let equiv (#g:env) (#g_card:env_card g) (t:typ) (fs_e:fs_env g_card -> elab_typ t) (e:exp) : Type0 =
+let equiv (#g:env) (t:typ) (fs_e:fs_env g -> elab_typ t) (e:exp) : Type0 =
   fv_in_env g e /\
-  forall b (s:gsub g g_card b) (fs_s:fs_env g_card).
+  forall b (s:gsub g b) (fs_s:fs_env g).
     s ∽ fs_s ==>  t ⦂ (fs_e fs_s, gsubst s e)
 
-let (≈) (#g:env) (#g_card:env_card g) (#t:typ) (fs_v:fs_env g_card -> elab_typ t) (e:exp) : Type0 =
-  equiv #g #g_card t fs_v e
+let (≈) (#g:env) (#t:typ) (fs_v:fs_env g -> elab_typ t) (e:exp) : Type0 =
+  equiv #g t fs_v e
 
 (** Equiv closed terms **)
 let equiv_closed_terms (#t:typ) (fs_e:elab_typ t) (e:closed_exp) :
-  Lemma (requires equiv #empty #0 t (fun _ -> fs_e) e)
+  Lemma (requires equiv #empty t (fun _ -> fs_e) e)
         (ensures  t ⦂ (fs_e, e)) =
-  eliminate forall b (s:gsub empty 0 b) (fs_s:fs_env #empty 0).
+  eliminate forall b (s:gsub empty b) (fs_s:fs_env empty).
     s ∽ fs_s ==>  t ⦂ ((fun _ -> fs_e) fs_s, gsubst s e) with true gsub_empty fs_empty
 
 (** Rules **)
 
-let equiv_unit #g (g_card:env_card g)
-  : Lemma ((fun (_:fs_env g_card) -> ()) `equiv TUnit` EUnit)
-  = assert ((fun (_:fs_env g_card) -> ()) `equiv TUnit` EUnit) by (explode ())
+let equiv_unit g
+  : Lemma ((fun (_:fs_env g) -> ()) `equiv TUnit` EUnit)
+  = assert ((fun (_:fs_env g) -> ()) `equiv TUnit` EUnit) by (explode ())
 
-let equiv_true #g (g_card:env_card g)
-  : Lemma ((fun (_:fs_env g_card) -> true) `equiv TBool` ETrue)
-  = assert ((fun (_:fs_env g_card) -> true) `equiv TBool` ETrue) by (explode ())
+let equiv_true g
+  : Lemma ((fun (_:fs_env g) -> true) `equiv TBool` ETrue)
+  = assert ((fun (_:fs_env g) -> true) `equiv TBool` ETrue) by (explode ())
 
-let equiv_false #g (g_card:env_card g)
-  : Lemma ((fun (_:fs_env g_card) -> false) `equiv TBool` EFalse)
-  = assert ((fun (_:fs_env g_card) -> false) `equiv TBool` EFalse) by (explode ())
+let equiv_false g
+  : Lemma ((fun (_:fs_env g) -> false) `equiv TBool` EFalse)
+  = assert ((fun (_:fs_env g) -> false) `equiv TBool` EFalse) by (explode ())
 
-let equiv_var #g (g_card:env_card g) (x:var{x < g_card})
-  : Lemma ((fun (fs_s:fs_env g_card) -> get_v fs_s (var_to_fs g_card x)) ≈ EVar x)
-  = assert ((fun (fs_s:fs_env g_card) -> get_v fs_s (var_to_fs g_card x)) ≈ EVar x) by (explode ())
+let equiv_var g (x:var{Some? (g x)})
+  : Lemma ((fun (fs_s:fs_env g) -> get_v fs_s x) ≈ EVar x)
+  = assert ((fun (fs_s:fs_env g) -> get_v fs_s x) ≈ EVar x) by (explode ())
 
-let equiv_lam #g (g_card:env_card g) (t1:typ) (body:exp) (t2:typ) (f:fs_env g_card -> elab_typ (TArr t1 t2)) : Lemma
-  (requires (fun (fs_s:fs_env #(extend t1 g) (g_card+1)) -> f (fs_shrink #t1 fs_s) (get_v fs_s g_card)) ≈ body)
+let equiv_lam g (t1:typ) (body:exp) (t2:typ) (f:fs_env g -> elab_typ (TArr t1 t2)) : Lemma
+  (requires (fun (fs_s:fs_env (extend t1 g)) -> f (fs_shrink #t1 fs_s) (get_v fs_s 0)) ≈ body)
             // the asymmetry is here. body is an open expression, while for f, I don't have an open expression
             // the equiv is quantifying over the free variable of body, but not get_v
   (ensures f ≈ (ELam body)) =
   let g' = extend t1 g in
-  let g_card' : env_card g' = g_card + 1 in
   assume (fv_in_env g (ELam body));
-  introduce forall b (s:gsub g g_card b) fs_s. s ∽ fs_s ==> TArr t1 t2 ⦂ (f fs_s, gsubst s (ELam body)) with begin
+  introduce forall b (s:gsub g b) fs_s. s ∽ fs_s ==> TArr t1 t2 ⦂ (f fs_s, gsubst s (ELam body)) with begin
     introduce _ ==> _ with _. begin
       let body' = subst (sub_elam s) body in
       assert (gsubst s (ELam body) == ELam body');
@@ -153,12 +142,12 @@ let equiv_lam #g (g_card:env_card g) (t1:typ) (body:exp) (t2:typ) (f:fs_env g_ca
         introduce _ ==> _ with _. begin
           let s' = gsub_extend s t1 v in
           let fs_s' = fs_extend fs_s fs_v in
-          eliminate forall b (s':gsub g' g_card' b) fs_s'. s' ∽ fs_s' ==>  t2 ⦂ (f (fs_shrink #t1 fs_s') (get_v fs_s' g_card), (gsubst s' body))
+          eliminate forall b (s':gsub g' b) fs_s'. s' ∽ fs_s' ==>  t2 ⦂ (f (fs_shrink #t1 fs_s') (get_v fs_s' 0), (gsubst s' body))
             with false s' fs_s';
           assert (s ∽ fs_s);
           assert (gsub_extend s t1 v ∽ fs_extend fs_s fs_v);
-          assert (t2 ⦂ (f (fs_shrink fs_s') (get_v fs_s' g_card), (gsubst s' body)));
-          assert (get_v (fs_extend fs_s fs_v) g_card == fs_v);
+          assert (t2 ⦂ (f (fs_shrink fs_s') (get_v fs_s' 0), (gsubst s' body)));
+          assert (get_v (fs_extend fs_s fs_v) 0 == fs_v);
           assert (t2 ⦂ (f (fs_shrink fs_s') fs_v, (gsubst s' body)));
           assert (t2 ⦂ (f fs_s fs_v, (gsubst s' body)));
           assume ((subst (sub_beta v) (subst (sub_elam s) body)) == (subst (gsub_extend s t1 v) body)); (** substitution lemma **)
@@ -171,13 +160,13 @@ let equiv_lam #g (g_card:env_card g) (t1:typ) (body:exp) (t2:typ) (f:fs_env g_ca
     end
   end
 
-let equiv_app #g (g_card:env_card g) (t1:typ) (t2:typ) (e1:exp) (e2:exp) (fs_e1:fs_env g_card -> elab_typ (TArr t1 t2)) (fs_e2:fs_env g_card -> elab_typ t1) : Lemma
+let equiv_app g (t1:typ) (t2:typ) (e1:exp) (e2:exp) (fs_e1:fs_env g -> elab_typ (TArr t1 t2)) (fs_e2:fs_env g -> elab_typ t1) : Lemma
   (requires fs_e1 ≈ e1 /\ fs_e2 ≈ e2)
   (ensures (fun fs_s -> (fs_e1 fs_s) (fs_e2 fs_s)) ≈ (EApp e1 e2)) =
   assert (fv_in_env g e1);
   assert (fv_in_env g e2);
   assume (fv_in_env g (EApp e1 e2)); (** should be proveable **)
-  introduce forall b (s:gsub g g_card b) fs_s. s ∽ fs_s ==> t2 ⦂ ((fs_e1 fs_s) (fs_e2 fs_s), gsubst s (EApp e1 e2)) with begin
+  introduce forall b (s:gsub g b) fs_s. s ∽ fs_s ==> t2 ⦂ ((fs_e1 fs_s) (fs_e2 fs_s), gsubst s (EApp e1 e2)) with begin
     let fs_e1' = fs_e1 fs_s in
     let fs_e2' = fs_e2 fs_s in
     let fs_e = fs_e1' fs_e2' in
@@ -197,14 +186,14 @@ let equiv_app #g (g_card:env_card g) (t1:typ) (t2:typ) (e1:exp) (e2:exp) (fs_e1:
     end
   end
 
-let equiv_if #g (g_card:env_card g) (t:typ) (e1:exp) (e2:exp) (e3:exp) (fs_e1:fs_env g_card -> elab_typ TBool) (fs_e2:fs_env g_card -> elab_typ t) (fs_e3:fs_env g_card -> elab_typ t) : Lemma
+let equiv_if g (t:typ) (e1:exp) (e2:exp) (e3:exp) (fs_e1:fs_env g -> elab_typ TBool) (fs_e2:fs_env g -> elab_typ t) (fs_e3:fs_env g -> elab_typ t) : Lemma
   (requires fs_e1 ≈ e1 /\ fs_e2 ≈ e2 /\ fs_e3 ≈ e3)
   (ensures (fun fs_s -> if fs_e1 fs_s then fs_e2 fs_s else fs_e3 fs_s) ≈ EIf e1 e2 e3) =
   assert (fv_in_env g e1);
   assert (fv_in_env g e2);
   assert (fv_in_env g e3);
   assume (fv_in_env g (EIf e1 e2 e3)); (** should be proveable **)
-  introduce forall b (s:gsub g g_card b) fs_s. s ∽ fs_s ==> t ⦂ ((if fs_e1 fs_s then fs_e2 fs_s else fs_e3 fs_s), gsubst s (EIf e1 e2 e3)) with begin
+  introduce forall b (s:gsub g b) fs_s. s ∽ fs_s ==> t ⦂ ((if fs_e1 fs_s then fs_e2 fs_s else fs_e3 fs_s), gsubst s (EIf e1 e2 e3)) with begin
     let fs_e1' = fs_e1 fs_s in
     let fs_e2' = fs_e2 fs_s in
     let fs_e3' = fs_e3 fs_s in
